make more progress on pip

priority.lean
@@ -1,8 +1,11 @@
-set_option pp.fieldNotation false
+set_option pp.fieldNotation true
 
 inductive Kind where
   | proc : Kind
   | lock : Kind
+
+open Kind
+axiom distinct_kind : lock ≠ proc
 
 structure St (world_size : Nat) where
   pto: Option (Fin world_size)
@@ -15,21 +18,80 @@ def St.curr_prio (s : St n) : Nat :=
   | none => s.def_prio
   | some m => max m s.def_prio
 
-structure World where
-  size : Nat
+structure World (size : Nat) where
   store : Array (St size)
-  invariant : store.size = size
-  pf_ptr : ∀ (i : Fin size), match store[i].pto with
-                              | none => true
-                              | some pto => store[i].kind ≠ store[pto].kind
+  -- this is by definition
+  pf_sz : store.size = size
+  -- valid, easy to prove
+  pf_idx : (i : Fin size) → (h : store.size = size) → i < store.size
+  -- invariant
+  pf_ptr : (i : Fin size)
+    → (h : (store[i]'(pf_idx i pf_sz)).pto = some pto)
+    → (store[i]'(pf_idx i pf_sz)).kind ≠ (store[pto]'(pf_idx pto pf_sz)).kind
 
-def World.acquire (w : World) (p_i r_i : Fin w.store.size) {p_k : w.store[p_i].kind = proc} {r_k : w.store[r_i].kind = lock} : World :=
-  have _ : p_i < w.size := by sorry
-  have _ : r_i < w.size := by sorry
+theorem World.no_self_ptr {size : Nat} {w : World size}
+  : ((i : Fin size) → (w.store[i]'(w.pf_idx i w.pf_sz)).pto ≠ some i) := by
+  sorry
+
+def World.acquire {wsize : Nat} (w : World wsize)
+  (p_i r_i : Fin wsize)
+  {p_k : (w.store[p_i]'(w.pf_idx p_i w.pf_sz)).kind = proc}
+  {r_k : (w.store[r_i]'(w.pf_idx r_i w.pf_sz)).kind = lock} : World wsize :=
+
+  have _ : p_i < w.store.size := w.pf_idx p_i w.pf_sz
+  have _ : r_i < w.store.size := w.pf_idx r_i w.pf_sz
+
+  have pf_p_ne_r : p_i ≠ r_i := by
+    intro h
+    have _ : lock = proc := by
+      calc lock
+      _ = w.store[r_i].kind := by rw [r_k]
+      _ = w.store[p_i].kind := by simp [h]
+      _ = proc := p_k
+    contradiction
 
   let p := w.store[p_i]
   let r := w.store[r_i]
 
-  w
+  match r.pto with
+  | none =>
+    let res := {w.store[r_i] with pto := some p_i}
+    have r_set : r_i < w.store.size := by simp [w.pf_sz]
 
-def World.update (w : World) (fr to : Nat) {_ : to >= fr} : World := sorry
+    let store := w.store.set (Fin.mk r_i r_set) res
+
+    have pf_res_kind : res.kind = w.store[r_i].kind := by rfl
+    have pf_res_pto : res.pto = some p_i := by rfl
+
+    have pf_sz : store.size = wsize := by
+      unfold store
+      rw [Array.size_set, w.pf_sz]
+
+    have pf_store_ri : store[r_i] = res := by sorry
+    have pf_store_ri_pto : store[r_i].pto = some p_i := by simp [pf_store_ri]
+
+    have _ := w.pf_sz
+    have pf_store_eq_1 : (i : Fin wsize) -> i ≠ r_i → store[i] = w.store[i] := by sorry
+
+    have pf_idx : (i : Fin wsize) → (h : store.size = wsize) → i < store.size := by
+      intro i h
+      rw [h]
+      exact i.isLt
+
+    have pf_ptr {pto : Fin wsize} (i : Fin wsize) (h : store[i].pto = some pto)
+      : store[i].kind ≠ store[pto].kind := by
+      by_cases h1 : i = r_i
+      . simp [*] at *
+        rw [h]
+        sorry
+      . rw [pf_store_eq_1 i h1]
+        sorry
+
+    World.mk store pf_sz pf_idx pf_ptr -- new world
+  | some pto =>
+    if pto == p_i
+      -- resource already points to the process
+      then w
+      else sorry
+
+def World.update {wsize : Nat} (w : World wsize) (fr to : Nat) {_ : to >= fr} : World wsize := sorry
